Otway-Rees: implemented impersonate responder attack
Implemented the attack in which the attacker makes use of the fact that the server
does not verify whether the combination of conv. id and principal names in the
encrypted parts match the unencrypted part. Thus, the attacker can replace the
responder name in the unencrypted part and gets a key intended for the initiator
and him, while the initiator will believe it is for him and the actual responder
(that is not involved in the protocol run at all).

otway-rees/OYRS.Attacker.fst
@@ -6,7 +6,9 @@ open CryptoEffect
 open CryptoLib
 open GlobalRuntimeLib
 open LabeledRuntimeAPI
+open SecurityLemmas
 
+module M = OYRS.Messages
 module S = OYRS.Sessions
 module L = LabeledPKI
 module A = AttackerAPI
@@ -118,6 +120,146 @@ let attacker_intercept_msg_2 (srv bob:principal) (msg2_idx:nat) :
     let send_mal_m3_idx = A.send #now srv bob ser_msg3 in
 
     (send_mal_m3_idx, conv_key)
+  | Error e -> error e
+
+val query_secret_key: idx_state:nat -> idx_corrupt:nat -> idx_query:nat ->
+    p:principal -> si:nat -> vi:nat ->
+    LCrypto (A.pub_bytes idx_query) (L.pki S.oyrs_preds)
+    (requires (fun t0 -> idx_state < idx_query /\ idx_corrupt < idx_query /\ idx_query <= trace_len t0 /\ was_corrupted_at idx_corrupt p si vi))
+    (ensures (fun t0 _ t1 -> t1 == t0))
+
+let query_secret_key idx_state idx_corrupt idx_query p si vi =
+  let ser_st = A.query_state_i idx_state idx_corrupt idx_query p si vi in
+  match
+    A.split ser_st `bind` (fun (tag_bytes, rest) ->
+    A.pub_bytes_to_string tag_bytes `bind` (fun lpki_tag ->
+    match lpki_tag with
+    | "APP" ->
+      A.split rest `bind` (fun (tag_bytes, rest) ->
+      A.pub_bytes_to_string tag_bytes `bind` (fun oyrs_tag ->
+      match oyrs_tag with
+      | "r_init" ->
+        A.split rest `bind` (fun (srv_bytes, k_es) ->
+        Success k_es)
+      | "r_sent_m2" ->
+        A.split rest `bind` (fun (srv_bytes, rest) ->
+        A.split rest `bind` (fun (k_es, _) ->
+        Success k_es))
+      | t -> Error ("query_secret_key: wrong oyrs session state tag: " ^ t ^ "\n")
+      ))
+    | t -> Error ("query_secret_key: wrong lpki session state tag: " ^ t ^ "\n")
+    ))
+  with Success k -> k | Error e -> error e
+
+let attacker_send_mal_msg_2 (#i:nat) (eve srv:principal) (msg1_idx:nat)
+  (k_es:A.pub_bytes i) :
+  Crypto (timestamp * g_trace)
+         (requires (fun t0 -> i <= trace_len t0 /\ msg1_idx < trace_len t0))
+         (ensures (fun t0 r t1 ->
+         match r with
+         | Error _ -> (t0 == t1 \/
+           (A.attacker_modifies_trace t0 t1 /\
+           later_than (trace_len t1) (trace_len t0)))
+         | Success (n, t01) ->
+           trace_len t1 = trace_len t0 + 3 /\
+           later_than (trace_len t1) (trace_len t0) /\
+           n = trace_len t1 - 1 /\
+           A.attacker_modifies_trace t0 t01 /\
+           A.attacker_modifies_trace t01 t1))
+= // receive and parse first message
+  let (|t_m1,ser_msg1|) = A.receive_i msg1_idx eve in
+
+  match
+    A.split ser_msg1 `bind` (fun (tag_bytes, rest) ->
+    A.pub_bytes_to_string tag_bytes `bind` (fun tag ->
+    match tag with
+    | "msg1" ->
+      A.split rest `bind` (fun (c, rest) ->
+      A.split rest `bind` (fun (a_bytes, rest) ->
+      A.split rest `bind` (fun (b_bytes, ev_a) ->
+      Success (c,a_bytes,b_bytes,ev_a))))
+    | t -> Error ("attacker_send_mal_m2: wrong message: " ^ t ^ "\n")
+    ))
+  with
+  | Success (c,a_bytes,b_bytes,c_ev_a) ->
+    // generate "responder" nonce
+    let (|now,n_e|) = A.pub_rand_gen (nonce_usage "nonce_attacker") in
+    let intermediate_trace = get () in
+
+
+    // create and send malicious second message. Muhahah
+    let c = A.pub_bytes_later t_m1 now c in
+    let a_bytes = A.pub_bytes_later t_m1 now a_bytes in
+    let b_bytes = A.pub_bytes_later t_m1 now b_bytes in
+    let e_bytes = A.pub_bytes_later 0 now (A.string_to_pub_bytes eve) in
+    let c_ev_a = A.pub_bytes_later t_m1 now c_ev_a in
+
+    let ev2 = A.concat n_e (A.concat c (A.concat a_bytes b_bytes)) in
+    let k_es = A.pub_bytes_later i now k_es in
+    let iv = A.pub_bytes_later 0 now (A.string_to_pub_bytes "iv") in
+    let ad = A.pub_bytes_later 0 now (A.string_to_pub_bytes "ev_r") in
+    let c_ev2 = A.aead_enc #now k_es iv ev2 ad in
+
+    let msg2_tag = A.pub_bytes_later 0 now (A.string_to_pub_bytes "msg2") in
+    let ser_msg2 = A.concat msg2_tag (A.concat c (A.concat a_bytes (A.concat e_bytes (A.concat c_ev_a c_ev2)))) in
+
+    let send_mal_m2_idx = A.send #now eve srv ser_msg2 in
+
+    (send_mal_m2_idx, intermediate_trace)
+  | Error e -> error e
+
+let attacker_send_msg_4 (#i:nat) (eve bob alice:principal) (msg3_idx:nat)
+  (k_es:A.pub_bytes i) :
+  Crypto (timestamp * bytes)
+         (requires (fun t0 -> i < trace_len t0 /\ msg3_idx < trace_len t0))
+         (ensures (fun t0 r t1 ->
+         match r with
+         | Error _ -> t0 == t1
+         | Success (n, b) ->
+           A.attacker_modifies_trace t0 t1 /\
+           trace_len t1 = trace_len t0 + 1 /\
+           later_than (trace_len t1) (trace_len t0) /\
+           n = trace_len t0 /\
+           A.attacker_knows_at n b))
+= // receive and parse third message
+  let (|t_m3,ser_msg3|) = A.receive_i msg3_idx eve in
+
+  match
+    A.split ser_msg3 `bind` (fun (tag_bytes, rest) ->
+    A.pub_bytes_to_string tag_bytes `bind` (fun tag ->
+    match tag with
+    | "msg3" ->
+      A.split rest `bind` (fun (c, rest) ->
+      A.split rest `bind` (fun (ev_a, ev_e) ->
+      Success (c,ev_a,ev_e)))
+    | t -> Error ("attacker_send_m4: wrong message: " ^ t ^ "\n")
+    ))
+  with
+  | Success (c,c_ev_a,c_ev_e) -> (
+    // decrypt part "intended" for attacker and extract conversation key
+    let now = global_timestamp () in
+    let c_ev_e = A.pub_bytes_later t_m3 now c_ev_e in
+    let k_es = A.pub_bytes_later i now k_es in
+    let iv = A.pub_bytes_later 0 now (A.string_to_pub_bytes "iv") in
+    let ad = A.pub_bytes_later 0 now (A.string_to_pub_bytes "ev_r") in
+    match
+      A.aead_dec #now k_es iv c_ev_e ad `bind` (fun ev_e ->
+      A.split ev_e `bind` (fun (_, k_ab) -> Success k_ab))
+    with
+    | Success k_ab -> (
+      //create and send fourth message
+      let c = A.pub_bytes_later t_m3 now c in
+      let c_ev_a = A.pub_bytes_later t_m3 now c_ev_a in
+
+      let msg4_tag = A.pub_bytes_later 0 now (A.string_to_pub_bytes "msg4") in
+      let ser_msg4 = A.concat msg4_tag (A.concat c c_ev_a) in
+
+      let send_m4_idx = A.send #now bob alice ser_msg4 in
+
+      (send_m4_idx, k_ab)
+    )
+    | Error e -> error e
+  )
   | Error e -> error e
 
 /// The instantiation of this lemma requires that the attacker knows `conv_key`.
